update Chap10 Sec06

Fpil/Chap10/Sec06.lean
@@ -71,3 +71,70 @@ def insertionSort [Ord α] (arr : Array α) : Array α :=
 
 #eval insertionSort #[3, 1, 7, 4]
 #eval insertionSort #[ "quartz", "marble", "granite", "hematite"]
+
+def insertSorted' [Ord α] (arr : Array α) (i : Fin arr.size) : Array α :=
+  match i with
+  | ⟨0, _⟩ => arr
+  | ⟨i' + 1, _⟩ =>
+    have : i' < arr.size := by
+      simp [Nat.lt_of_succ_lt, *]
+    match Ord.compare arr[i'] arr[i] with
+    | .lt | .eq => arr
+    | .gt =>
+      insertSorted'
+        ((dbgTraceIfShared "array to swap" arr).swap ⟨i', by assumption⟩ i)
+        ⟨i', by simp [dbgTraceIfShared, *]⟩
+
+theorem insert_sorted_size_eq' [Ord α] (len : Nat) (i : Nat) :
+  (arr : Array α) → (isLt : i < arr.size) → (arr.size = len) →
+  (insertSorted' arr ⟨i, isLt⟩).size = len := by
+  induction i with
+  | zero =>
+    intro arr isLt hLen
+    simp [insertSorted', *]
+  | succ i' ih =>
+    intro arr isLt hLen
+    simp [insertSorted', dbgTraceIfShared]
+    split <;> simp [*]
+
+def insertionSortLoop' [Ord α] (arr : Array α) (i : Nat) : Array α :=
+  if h : i < arr.size then
+    have : (insertSorted' arr ⟨i, h⟩).size - (i + 1) < arr.size - i := by
+      rw [insert_sorted_size_eq' arr.size i arr h rfl]
+      simp [Nat.sub_succ_lt_self, *]
+    insertionSortLoop' (insertSorted' arr ⟨i, h⟩) (i + 1)
+  else
+    arr
+termination_by insertionSortLoop' arr i => arr.size - i
+
+def insertionSort' [Ord α] (arr : Array α) : Array α :=
+  insertionSortLoop' arr 0
+
+#eval insertionSort' #[3, 1, 7, 4]
+#eval insertionSort' #[ "quartz", "marble", "granite", "hematite"]
+
+
+def getLines : IO (Array String) := do
+  let stdin ← IO.getStdin
+  let mut lines : Array String := #[]
+  let mut currLine ← stdin.getLine
+  while !currLine.isEmpty do
+    lines := lines.push (currLine.dropRight 1)
+    currLine ← stdin.getLine
+  pure lines
+
+def mainUnique : IO Unit := do
+  let lines ← getLines
+  for line in insertionSort' lines do
+    IO.println line
+
+def mainShared : IO Unit := do
+  let lines ← getLines
+  IO.println "--- Sorted lines: ---"
+  for line in insertionSort' lines do
+    IO.println line
+  --
+  IO.println ""
+  IO.println "--- Original data: ---"
+  for line in lines do
+    IO.println line
